vera/VerilogToSMT/VerilogToSMT.v
@@ -168,10 +168,12 @@ Section expr_to_smt.
   .
 
   Equations transfer_module_item : Verilog.module_item -> transf (SMTLib.term Sort_Bool) :=
-    transfer_module_item (Verilog.AlwaysComb (Verilog.BlockingAssign var rhs)) :=
+    transfer_module_item (Verilog.AlwaysComb (Verilog.BlockingAssign (Verilog.AssignVar var) rhs)) :=
       let lhs_smt := var_to_smt var in
       let* rhs_smt := expr_to_smt rhs in
       ret (SMTLib.Term_Eq lhs_smt rhs_smt);
+    transfer_module_item (Verilog.AlwaysComb (Verilog.BlockingAssign _ _)) :=
+      raise "Unexpected assign LHS in VerilogToSMT stage"%string;
   .
 
   Equations transfer_module_body : list Verilog.module_item -> transf (list (SMTLib.term Sort_Bool)) :=
